theories/once.v
@@ -1,0 +1,49 @@
+From det Require Import prelude.
+From mathcomp Require Import all_ssreflect.
+From det Require Import tree tree_prop ctx.
+From det Require Import tree_prop_hard.
+
+From det Require Import check_fo.
+
+Section once.
+  Variable once_sym: P.
+  Definition once := 
+    let X := Tm_V 0 in
+  {| 
+    head := Callable_App (Callable_P once_sym) X;
+    premises := [::call ()]
+    
+  |}
+
+  Definition prog_once p :=
+    p.(rules) = []
+
+
+
+End once.
+
+Definition once := [::cut].
+
+
+Lemma is_det_tail_cut u p s fv l:
+  is_det u p s fv (And l [::cut] (And (TA cut) [::] OK)).
+Proof.
+  move=> b s' tx fv' H.
+  remember (And _ _ _) as t' eqn:Ht'.
+  elim_run H l Ht'.
+  - by move: SA; rewrite rew_pa => /andP[]//.
+  - move: pA eA; rewrite rew_pa/= !push.
+    case: ifP => sl pA [???]; subst.
+    rewrite -success_cut in sl.
+    inversion rB; subst => //=.
+    - rewrite sl next_alt_cutl//.
+    - move: H0 => /=; rewrite sl => -[???]; subst.
+      by move: H; rewrite rew_pa sl//.
+    - move: H; rewrite rew_pa sl success_failed//.
+  - by apply: IH erefl.
+  - move: fA nA; rewrite rew_pa/=.
+    move=> /orP[fl|/andP[]]//.
+    rewrite fl failed_success//.
+    case nl: next_alt => //=[l'][?]; subst. 
+    apply: IH erefl.
+Qed.
